Added better error messages, with locations

compiler/lexer.mll
@@ -48,4 +48,4 @@ rule token = parse
   | ['0'-'9' '_']+ as id { NUM (int_of_string id) }
   | ['A'-'Z' 'a'-'z'] ['A'-'Z' 'a'-'z' '0'-'9' '_']* as id { IDENT id }
   | _
-    { raise (Error (Printf.sprintf "At offset %d: unexpected character.\n" (Lexing.lexeme_start lexbuf))) }
+    { raise (Error (Format.sprintf "At offset %d: unexpected character.\n" (Lexing.lexeme_start lexbuf))) }
