compiler/locationInfo.ml
@@ -1,0 +1,27 @@
+type position = string * int * int
+let pp_position fmt ((f, l, c): position) =
+  Format.fprintf fmt "%s:%i:%i" f l c
+let position_of_lexerpos (p: Lexing.position): position = (p.pos_fname, p.pos_lnum, p.pos_cnum - p.pos_bol + 1)
+
+type extent = position * position
+
+let extent_of_len (len: int) (p: Lexing.position) =
+  let ((f, l, c) as e) = position_of_lexerpos p in ((f, l, c - len), e)
+
+let pp_extent fmt ((f1, l1, c1), (f2, l2, c2): extent) =
+  if f1 = f2 then
+    if l1 = l2 then
+      if c1 = c2 then
+        Format.fprintf fmt "%s:%i:%i" f1 l1 c1
+      else
+        Format.fprintf fmt "%s:%i:%i-%i" f1 l1 c1 c2
+    else
+      Format.fprintf fmt "%s:%i:%i-%i:%i" f1 l1 c1 l2 c2
+  else
+    Format.fprintf fmt "%s:%i:%i-%s:%i:%i" f1 l1 c1 f2 l2 c2
+
+let extend_to_pos (e: extent) (p: Lexing.position): extent = (fst e, position_of_lexerpos p)
+let extend_to_ext (e1: extent) (e2: extent): extent = (fst e1, snd e2)
+
+let extent_of_loc (fn: string) (l: Extracted.Result.location): extent =
+  ((fn, l.loc_start_line, l.loc_start_col), (fn, l.loc_end_line, l.loc_end_col))
