theories/Datatypes/Result.v
@@ -2,32 +2,79 @@ From Reactive Require Export Base.
 
 From Stdlib Require Export String.
 
+Record location : Set := {
+  loc_start_line: nat;
+  loc_start_col: nat;
+  loc_end_line: nat;
+  loc_end_col: nat;
+}.
 
-Inductive t (A: Type): Type :=
-  | Ok: A -> t A
-  | Err: string -> t A.
+Inductive declaration_location: Set :=
+  | DeclInput
+  | DeclOutput
+  | DeclLocal
+.
 
-Arguments Ok {_}.
-Arguments Err {_}.
+Inductive r {type: Set} | : Set :=
+  | BadType (expected: list type) (got: type): r
+  | IncompatibleTypeAssignment (vname: ident) (vtype: type) (etype: type): r
+  | UndeclaredInput (vname: ident): r
+  | UndeclaredVariable (vname: ident): r
+  | NeverAssigned (vname: ident) (vtype: type): r
+  | MultipleDeclaration (vname: ident) (loc1 loc2: declaration_location): r
+  | InternalError (msg: string): r
+.
+Arguments r _ : clear implicits.
+
+Inductive t type (A: Type) | : Type :=
+  | Ok: A -> t
+  | Err: list (location * r type) -> t.
+
+Arguments Ok [_] {_}.
+Arguments Err {_ _}.
 
 
-Definition bind {A B} (x: t A) (f: A -> t B): t B :=
+Definition combine_prop {type} {A B : Prop} (x: t type A) (y: t type B): t type (A /\ B) := match x, y with
+  | Ok x, Ok y => Ok (conj x y)
+  | Err x, Ok _ => Err x
+  | Ok _, Err y => Err y
+  | Err x, Err y => Err (x ++ y)
+end.
+
+Definition combine {type A B} (x: t type A) (y: t type B): t type (A * B) := match x, y with
+  | Ok x, Ok y => Ok (x, y)
+  | Err x, Ok _ => Err x
+  | Ok _, Err y => Err y
+  | Err x, Err y => Err (x ++ y)
+end.
+
+Definition bind {type A B} (x: t type A) (f: A -> t type B): t type B :=
   match x with
   | Err msg => Err msg
   | Ok x => f x
   end.
 
-Definition strong_bind {A B} (x: t A) (f: forall a: A, x = Ok a -> t B): t B :=
+Definition strong_bind {type A B} (x: t type A) (f: forall a: A, x = Ok a -> t type B): t type B :=
   match x as y return x = y -> _ with
   | Err msg => fun _ => Err msg
   | Ok x => f x
   end eq_refl.
 
+Definition list_map {type A} {P : A -> Prop} (dec : forall x, t type (P x)): forall l, t type (Forall P l) :=
+  fix inner l := match l with
+  | [] => Ok (Forall_nil _)
+  | hd :: tl => match dec hd with
+      | Ok H => bind (inner tl) (fun IH => Ok (Forall_cons _ H IH))
+      | Err es => Err (match inner tl with Ok _ => es | Err es' => es ++ es' end)
+      end
+  end.
+
 
 Module notations.
 
-  Notation "e1 >>= e2" := (bind e1 e2) (at level 60, right associativity).
+  Infix ">>=" := bind (at level 60, right associativity).
   Notation "'do' x <- e1 ; e2" := (bind e1 (fun x => e2)) (at level 60, x binder, right associativity).
   Notation "'do' x 'remember' e <- e1 ; e2" := (strong_bind e1 (fun x e => e2)) (at level 60, x binder, e binder, right associativity).
+  Infix ">+<" := combine (at level 60, right associativity).
 
 End notations.
